coq/denot/continuity.v
@@ -1,0 +1,670 @@
+(* 
+
+This section proves that the denotation function is monotonic and continuous.
+
+Monotonicity
+
+   Definition monotone (F : P Value -> P Value) : Set := 
+         forall D1 D2, (D1 ⊆ D2) -> F D1 ⊆ F D2.
+
+   Lemma denot_monotone_one : forall ρ t x, 
+    uniq ρ -> x `notin` dom ρ ->
+    monotone (fun D => denot (t ^ x) (x ~ D ++ ρ)).
+
+Continuity:
+
+   A semantic function is continuous if its finite result can be produced
+   by a finite and valid subset of its input.
+   
+   Definition continuous (F : P Value -> P Value) : Set :=
+     forall X E, mem E ⊆ F X -> valid X ->
+                 exists D, (mem D ⊆ X) /\ ((mem E) ⊆ F (mem D)) /\ valid_mem D.
+
+   Lemma denot_continuous_one { t ρ x } :
+     valid_env ρ ->
+     x `notin` dom ρ ->
+     continuous (fun D => denot (t ^ x) (x ~ D ++ ρ)).
+
+The payoff for this section is a lemma for understanding how LAMBDA and APPLY interact.
+The general lemma looks like this:
+
+Lemma Λ_APPLY_id { F X } :
+  continuous F -> monotone F -> valid X ->
+  (Λ F) ▩ X ≃ F X.
+
+With the above results, we can instantiate it to reason about the denotation function.
+
+Lemma Λ_denot_APPLY_id : forall t ρ x X,
+    valid X ->
+    valid_env ρ ->
+    x `notin` dom ρ ->
+    ((Λ (fun D => denot (t ^ x) (x ~ D ++ ρ))) ▩ X) ≃ denot (t ^ x) (x ~ X ++ ρ).
+
+ *)
+Require Import Coq.Logic.FunctionalExtensionality.
+Require Import Coq.Classes.RelationClasses.
+Require Coq.Relations.Relation_Definitions.
+Require Import Lia.
+
+Require Export lc.tactics.
+Require Import structures.Structures.
+
+Require Import denot.definitions.
+Require Import denot.denot.
+Require Import denot.congruence_theory.
+Require Import denot.valid_theory.
+
+Import MonadNotation.
+Open Scope monad_scope.
+Import SetNotations.
+Local Open Scope set_scope.
+Import LCNotations.
+Open Scope tm.
+
+Import EnvNotations.
+
+(* Definitions related to continuity *)
+
+Definition monotone (F : P Value -> P Value) : Set := 
+  forall D1 D2, (D1 ⊆ D2) -> F D1 ⊆ F D2.
+
+Definition finite (X : P Value) : Prop := 
+  exists E, (X ≃ mem E) /\ E <> nil.
+
+Definition continuous (F : P Value -> P Value) : Set :=
+  forall X E, mem E ⊆ F X -> valid X 
+         -> exists D, (mem D ⊆ X) /\ ((mem E) ⊆ F (mem D)) /\ valid_mem D.
+
+Definition monotone_env (D : Rho -> P Value) := 
+  forall ρ ρ' , ρ ⊆e ρ' -> (D ρ) ⊆ D ρ'.
+
+Definition finite_env : Rho -> Type := Env.ForallT finite.
+
+Definition continuous_In (D:Rho -> P Value) (ρ:Rho) (v:Value) : Prop :=
+  v ∈ D ρ -> exists ρ' , exists (pf : finite_env ρ'),  ρ' ⊆e ρ /\ (v ∈ D ρ').
+
+Definition continuous_env (D:Rho -> P Value) (ρ:Rho) : Prop :=
+  forall v, continuous_In D ρ v.
+
+(* -------------------------------------- *)
+
+
+Ltac gather_atoms ::=
+  let A := gather_atoms_with (fun x : vars => x) in
+  let B := gather_atoms_with (fun x : var => {{ x }}) in
+  let C := gather_atoms_with (fun x => fv_tm x) in
+  let D := gather_atoms_with (fun x : list (atom * P Value) => dom x) in
+  let E := gather_atoms_with (fun x : Rho => dom x) in
+  constr:(A \u B \u C \u D \u E).
+
+(* -------------------------------------- *)
+
+
+(* -- monotonicity -- *)
+
+Lemma access_monotone {ρ ρ':Rho}{x} : ρ ⊆e ρ' -> ρ ⋅ x ⊆ ρ' ⋅ x.
+Proof.
+  induction 1. simpl. reflexivity.
+  simpl. destruct (x == x0) eqn:E. auto.
+  auto. 
+Qed.
+
+(*  forall ρ ρ', ρ ⊆e ρ' -> denot t ρ ⊆ denot t ρ'. *)
+Lemma denot_monotone {t}: 
+  monotone_env (denot t).
+Proof.
+  unfold monotone_env.
+  eapply tm_induction with (t := t);
+  [move=>i|move=>y|move=>t1 t2 IH1 IH2|move=> t' IH|move=>k| | | move=> t1 t2 IH1 IH2].
+ all: intros ρ ρ' S.
+ all: autorewrite with denot.
+ all: try solve [reflexivity].
+  + eapply access_monotone; auto.
+  + eapply APPLY_mono_sub; eauto.
+  + pick fresh x.
+    repeat rewrite (denot_abs x).
+    fsetdec.
+    fsetdec.
+    eapply Λ_ext_sub.
+    intros X NE.
+    eapply IH. fsetdec.
+    eapply extend_sub_env; eauto. 
+  + eapply CONS_mono_sub; eauto.
+Qed.
+
+
+
+(* denot-monotone-one *)
+Lemma denot_monotone_one : forall ρ t x, 
+    uniq ρ -> x `notin` dom ρ ->
+    monotone (fun D => denot (t ^ x) (x ~ D ++ ρ)).
+Proof. 
+  intros.
+  unfold monotone. 
+  intros D1 D2 sub.
+  eapply denot_monotone; simpl; auto.
+  econstructor; eauto.
+Qed.
+  
+
+(* ----------------------------------------------------- *)
+
+(* Join environments *)
+
+Lemma join_finite_env {ρ1 ρ2} : 
+  same_scope ρ1 ρ2 
+  -> finite_env ρ1
+  -> finite_env ρ2
+  -> finite_env (ρ1 ⊔e ρ2).
+Proof.
+  move: ρ2.
+  induction ρ1 as [|[x1 v1] r1].
+  all: intros ρ2 sc h1; destruct ρ2 as [|[x2 v2] r2]; intros h2; simpl; eauto.
+  inversion h1; subst; clear h1.
+  inversion h2; subst; clear h2.
+  destruct (x1 == x2); subst.
+  + econstructor; eauto. eapply IHr1; eauto. inversion sc. auto.
+    rewrite sub_dom1; auto.
+    destruct H3 as [E1 [s1 u1 ]].
+    destruct H5 as [E2 [s2 u2 ]].
+    exists (E1 ++ E2).
+    split.
+    rewrite -> s1.
+    rewrite -> s2.
+    rewrite union_mem. reflexivity.
+    ++ intro h.
+    apply u2. 
+    destruct E1. simpl in h. auto.
+    done.
+  + assert False. inversion sc. subst. done. done.
+Qed.
+
+Lemma join_lub {ρ ρ1 : Rho} :
+  same_scope ρ1 ρ ->
+  forall ρ2, same_scope ρ2 ρ ->
+  ρ1 ⊆e ρ -> ρ2 ⊆e ρ -> (ρ1 ⊔e ρ2) ⊆e ρ.
+Proof.
+  intro SS1.
+  induction SS1; intros ρ2 SS2; inversion SS2; subst.
+  simpl. auto.
+  intros.
+  simpl.
+  inversion H1. inversion H2. subst.
+  rewrite eq_dec_refl.
+  eapply Env.Forall2_cons; eauto.
+  rewrite sub_dom1. auto.
+  rewrite -> H21.
+  rewrite -> H13.
+  rewrite union_idem.
+  reflexivity.
+Qed.
+  
+Lemma join_sub_left {ρ1 ρ2 : Rho} : 
+  same_scope ρ1 ρ2 ->
+  ρ1 ⊆e (ρ1 ⊔e ρ2).
+Proof.
+  intros h.
+  induction h; simpl; eauto.
+  rewrite eq_dec_refl.
+  econstructor; eauto. 
+Qed.
+
+Lemma join_sub_right {ρ1 ρ2 : Rho} : 
+  same_scope ρ1 ρ2 ->
+  ρ2 ⊆e (ρ1 ⊔e ρ2).
+Proof.
+  induction 1; simpl; eauto. 
+  rewrite eq_dec_refl.
+  econstructor; eauto. 
+  erewrite Forall2_dom in H0; eauto.
+Qed.
+
+(* --------------------------------------- *)
+
+(* Initial environment. *)
+
+(* creates an environment that maps each variable x to a singleton 
+   set of some element in ρ x *)
+Definition initial_finite_env (ρ : Rho) (NE : valid_env ρ) : Rho.
+  induction NE. exact nil.
+  destruct f as [[V _] _].
+  exact (cons (x, ⌈ V ⌉) IHNE).
+Defined.
+
+Lemma initial_finite_dom : forall E NE, dom (initial_finite_env E NE) = dom E.
+Proof.
+  induction NE; simpl. auto.
+  destruct f as [[v _] w].  simpl. congruence.
+Qed. 
+
+#[export] Hint Rewrite initial_finite_dom : rewr_list.
+
+Lemma finite_singleton : forall v, finite ⌈ v ⌉.
+Proof. intros v.  exists (cons v nil).
+       repeat split; eauto. done. 
+Qed.
+
+#[export] Hint Resolve finite_singleton : core. 
+
+
+Lemma initial_fin (ρ : Rho) (NE : valid_env ρ) :
+  finite_env (initial_finite_env ρ NE).
+Proof.
+  induction NE.
+  simpl. econstructor.
+  simpl. destruct f as [[v _] w1 ].
+  econstructor; eauto.
+  rewrite initial_finite_dom. auto.
+Qed.
+
+#[global] Hint Resolve initial_fin : core. 
+
+
+Lemma initial_fin_sub (ρ : Rho) (NE : valid_env ρ) :
+  initial_finite_env ρ NE ⊆e ρ.
+Proof.
+  induction NE; simpl. econstructor.
+  destruct f as [[v wpx] _].
+  econstructor. auto.
+  rewrite initial_finite_dom. auto.
+  intros z y. inversion y. subst. unfold In. auto.
+Qed.
+
+#[global] Hint Resolve initial_fin_sub : core. 
+
+
+(* single-env maps x to D and any other variable y to something in ρ y. *)
+Definition single_env (x : atom) (D : P Value) (ρ : Rho) 
+  (NE : valid_env ρ) : Rho :=
+  update x D (initial_finite_env ρ NE).
+
+  
+Lemma single_fin { v x ρ NE } : 
+  finite_env (single_env x ⌈ v ⌉ ρ NE).
+Proof.
+  induction NE; unfold finite_env; eauto.
+  unfold single_env; econstructor.
+  unfold single_env. simpl. 
+  destruct f as [[v1 I1] v2].
+  destruct (x == x0) eqn:EQ.
+  + subst. rewrite update_eq_var. 
+    econstructor.
+    eapply initial_fin. simpl_env. auto. auto.
+  + rewrite update_neq_var; eauto.
+    econstructor; eauto.
+    simpl_env. auto.
+Qed.
+
+#[global] Hint Resolve single_fin : core. 
+
+
+Lemma single_sub { ρ x v } :
+  forall (NE : valid_env ρ),
+    v ∈ ρ ⋅ x 
+  -> x `in` dom ρ
+  -> (single_env x ⌈ v ⌉ ρ NE) ⊆e ρ.
+Proof.
+  intros NE.
+  induction NE.
+  all: intros vpe Indom. 
+  + (* nil case *) auto. 
+  + (* cons case *)
+    unfold single_env in *.
+    simpl. simpl_env in Indom.
+    destruct f as [[w h1] h2]. simpl.
+    simpl in vpe.
+    destruct (x == x0).
+    ++ subst. econstructor; eauto.
+       simpl_env.  eauto.
+       intros x h. inversion h. subst. auto.
+    ++ econstructor; eauto. 
+       eapply IHNE; eauto. fsetdec.
+       simpl_env. auto.
+       intros y h. inversion h. subst. unfold In. auto.
+Qed.
+
+#[export] Hint Resolve single_sub : core. 
+
+
+(* v∈single[xv]x  *)
+Lemma v_single_xvx {v x ρ NE} : 
+  x `in` dom ρ ->
+  v ∈ (single_env x ⌈ v ⌉ ρ NE ⋅ x).
+Proof.
+  unfold single_env.
+  move: NE.
+  induction NE; intro h. fsetdec.
+  simpl. destruct f as [[w h1] h2]. simpl.
+  destruct (x == x0) eqn:EQ. subst. simpl.
+  rewrite eq_dec_refl. econstructor; eauto.
+  simpl. rewrite EQ. simpl in h. eapply IHNE; auto. fsetdec.
+Qed.  
+
+#[export] Hint Resolve v_single_xvx : core. 
+
+(* continuous-∈⇒⊆ *)
+Lemma continuous_In_sub E ρ (NE : valid_env ρ) :
+   monotone_env E
+   -> forall V, mem V ⊆ E ρ
+   -> (forall v, v ∈ mem V -> continuous_In E ρ v)
+   -> exists ρ', exists (pf : finite_env ρ') ,  ρ' ⊆e ρ /\ (mem V ⊆ E ρ').
+Proof.
+  intros me V VE vcont.
+  induction V.
+  - exists (initial_finite_env ρ NE).
+    repeat split.
+    eapply (initial_fin ρ NE).
+    eapply initial_fin_sub; eauto. 
+    done.
+  - destruct IHV as [ ρ1 [ fρ1 [ ρ1ρ VEρ1 ]]].
+    intros d z. eapply VE; eauto.
+    intros v VM. eapply vcont; eauto.
+    destruct (vcont a) as [ρ2 [fρ2 [ρ2ρ VEρ2]]].
+    econstructor; eauto.
+    eapply VE. econstructor; eauto.
+    exists (ρ1 ⊔e ρ2).
+    have S1: same_scope ρ1 ρ. eapply Forall2_same_scope; eauto.
+    have S2: same_scope ρ2 ρ. eapply Forall2_same_scope; eauto. 
+    have SS: same_scope ρ1 ρ2. 
+    { transitivity ρ; auto. symmetry; auto. }
+    eexists. eapply join_finite_env; eauto.
+    repeat split.
+    + eapply join_lub; eauto.
+    + intros d dm.
+    inversion dm; subst.
+    eapply me. eapply join_sub_right; eauto. auto. 
+    eapply me. eapply join_sub_left; eauto. auto.
+Qed.
+
+(* --------------------------------------- *)
+
+(* Operations are continuous *)
+
+
+Lemma CONS_continuous {D E ρ}{w} :
+    w ∈ (CONS (D ρ) (E ρ))
+  -> continuous_env D ρ 
+  -> continuous_env E ρ
+  -> monotone_env D 
+  -> monotone_env E
+  -> exists ρ3 , exists (pf : finite_env ρ3) , ρ3 ⊆e  ρ /\ (w ∈ (CONS (D ρ3) (E ρ3))).
+Proof.  
+  intros C. unfold CONS, In in C. destruct w.
+  all: try done.
+  destruct l. try done.
+  move: C => [Dv El].
+  intros IHD IHE mD mE.
+  destruct (IHD v Dv) as 
+      [ ρ1 [ fρ1 [ ρ1ρ VwDp1 ]]].
+  destruct (IHE (v_list l) El) as 
+      [ ρ2 [ fρ2 [ ρ2ρ VwDp2 ]]].
+  have S1: same_scope ρ1 ρ. eapply Forall2_same_scope; eauto.
+  have S2: same_scope ρ2 ρ. eapply Forall2_same_scope; eauto.
+  have SS: same_scope ρ1 ρ2. { transitivity ρ; auto. symmetry; auto. }
+  exists (ρ1 ⊔e ρ2).
+    repeat split.
+  - eapply join_finite_env; eauto.
+  - eapply join_lub; eauto.
+  - eapply mD. instantiate (1:= ρ1). 
+    eapply join_sub_left; eauto. auto.
+  - eapply mE. instantiate (1:= ρ2).
+    eapply join_sub_right; eauto. auto.
+Qed.
+
+
+Lemma APPLY_continuous {D E ρ}{w} :
+  (valid_env ρ)
+  -> w ∈ ((D ρ) ▩ (E ρ))
+  -> continuous_env D ρ 
+  -> continuous_env E ρ
+  -> monotone_env D 
+  -> monotone_env E
+  -> exists ρ3 , 
+    exists (pf : finite_env ρ3) , ρ3 ⊆e  ρ 
+                             /\ (w ∈ ((D ρ3) ▩ (E ρ3))).
+Proof.  
+  intros NE APP. inversion APP; subst. 
+  all: intros IHD IHE mD mE.
+  + destruct (IHD v_wrong H) as
+      [ ρ1 [ fρ1 [ ρ1ρ VwDp1 ]]].
+    exists ρ1. exists fρ1. split. auto.
+    eapply FUNWRONG; auto.
+  + destruct (IHE v_wrong H) as 
+      [ ρ1 [ fρ1 [ ρ1ρ VwDp1 ]]].
+    exists ρ1. exists fρ1. split. auto.
+    eapply ARGWRONG; auto.
+  + destruct (IHD (V ↦ w) H) as 
+      [ ρ1 [ fρ1 [ ρ1ρ VwDp1 ]]].
+    destruct 
+      (continuous_In_sub E ρ NE mE V)
+      as [ ρ2 [ fρ2 [ ρ2ρ VEp2 ]]]; eauto.
+    have S1: same_scope ρ1 ρ. eapply Forall2_same_scope; eauto.
+    have S2: same_scope ρ2 ρ. eapply Forall2_same_scope; eauto.
+    have SS: same_scope ρ1 ρ2. { transitivity ρ; auto. symmetry; auto. }
+    exists (ρ1 ⊔e ρ2).
+    repeat split.
+  - eapply join_finite_env; eauto.
+  - eapply join_lub; eauto.
+  - have VwDp3 : V ↦ w ∈ D (ρ1 ⊔e ρ2).
+    { eapply mD. 2: eapply VwDp1. 
+      eapply join_sub_left. auto. }
+    have VEρ3 : mem V ⊆ E (ρ1 ⊔e ρ2).
+    { intros v vV. eapply mE.
+      2: eapply VEp2; auto. 
+      eapply join_sub_right.  auto. }
+    eapply BETA with (V:=V); auto.
+ + destruct (IHD (v_list VS)) as [ρ1 [F1 [h1 h2]]]; auto.
+   destruct (IHE (v_nat k)) as [ρ2 [F2 [h3 h4]]]; auto.
+    have S1: same_scope ρ1 ρ. eapply Forall2_same_scope; eauto.
+    have S2: same_scope ρ2 ρ. eapply Forall2_same_scope; eauto.
+    have SS: same_scope ρ1 ρ2. { transitivity ρ; auto. symmetry; auto. }
+   exists (ρ1 ⊔e ρ2).
+    repeat split.
+  - eapply join_finite_env; eauto.    
+  - eapply join_lub; eauto.
+  - eapply PROJ with (VS := VS) (k:=k); eauto.
+    eapply mD. eapply join_sub_left; auto. auto.
+    eapply mE. eapply join_sub_right; auto. auto.
+ +  destruct (IHD x) as [ρ1 [F1 [h1 h2]]]; auto.
+    eexists.
+    eexists.
+    eauto.
+    split; eauto.
+    eapply APPWRONG with (x:=x); auto.
+ +  destruct (IHE x) as [ρ2 [F1 [h1 h2]]]; auto.
+    destruct (IHD (v_list VS)) as [ρ1 [F2 [h01 h02]]]; auto.
+    have S1: same_scope ρ1 ρ. eapply Forall2_same_scope; eauto.
+    have S2: same_scope ρ2 ρ. eapply Forall2_same_scope; eauto.
+    have SS: same_scope ρ1 ρ2. { transitivity ρ; auto. symmetry; auto. }
+    exists (ρ1 ⊔e ρ2).
+    repeat split.
+    - eapply join_finite_env; eauto.    
+    - eapply join_lub; eauto.
+    - eapply PROJWRONG with (VS := VS); eauto.
+    eapply mD. eapply join_sub_left; auto. auto.
+    eapply mE. eapply join_sub_right; auto. auto.
+Qed.
+
+
+
+Lemma env_tail {ρ' x v ρ} :  
+  ρ' ⊆e (x ~ v ++ ρ) -> finite_env ρ' -> 
+  nonempty_env ρ ->
+  exists w, exists ρ'', ρ' = (x ~ w ++ ρ'') /\
+                (w ⊆ v) /\
+                exists (pf : finite_env ρ''), 
+                ρ'' ⊆e ρ.                
+Proof.
+  intros h k ne.
+  inversion h. subst.
+  exists a1.  exists E1.
+  repeat split; auto. inversion k.  auto.
+Qed.
+
+(* Algebraicity.  
+   Only need finite information from the environment.
+*)
+
+Lemma Lambda_continuous {E ρ} {NE : valid_env ρ}{ v x} :
+  v ∈ Λ (fun D => E (x ~ D ++ ρ)) 
+  -> (forall V, valid_mem V -> continuous_env E (x ~ mem V ++ ρ))
+  -> monotone_env E
+  -> exists ρ', exists (pf:finite_env ρ'),
+            ρ' ⊆e ρ /\  (v ∈ (Λ (fun D => E (x ~ D ++ ρ')))).
+Proof.
+  induction v.
+  all: try solve [intros; cbv in H; done].
+  - (* v is l ↦ v *)
+    intros [ wEVρ [NW CL] ] IH mE.
+    have VV: valid_mem l. unfold valid_mem. split; eauto.
+    destruct (IH l ltac:(eauto) v wEVρ) as
+      [ ρ' [ fρ' [ ρ'Vρ wEρ' ]]]. 
+    inversion ρ'Vρ. subst. clear ρ'Vρ.
+    inversion fρ'. subst. clear fρ'.
+    exists E1. exists X.
+    repeat split; eauto.
+    eapply mE. 2: exact wEρ'.
+    have SS: E1 ⊆e E1. eapply Reflexive_sub_env.  eapply Forall2_uniq1; eauto. 
+    auto.
+  - exists (initial_finite_env ρ NE).
+    repeat split; eauto.
+Qed.
+
+
+(* ---------------- Denotation is continuous ----------------- *)
+
+
+(* ⟦⟧-continuous *)
+Lemma denot_continuous {t} : forall ρ,
+    valid_env ρ
+  -> continuous_env (denot t) ρ.
+Proof.
+  eapply tm_induction with (t := t);
+  [move=>i|move=>x|move=>t1 t2 IH1 IH2|move=> t' IH|move=>k| | | move=> t1 t2 IH1 IH2].
+  all: intros ρ NE.
+  all: intros v vIn.
+  all: autorewrite with denot in vIn.
+  all: try solve [ exists (initial_finite_env ρ NE);
+    eexists; eauto] .
+  + destruct (FSetDecideAuxiliary.dec_In x (dom ρ)).
+    - exists (single_env x ⌈ v ⌉ ρ NE).
+      exists (@single_fin v x ρ NE).
+      split.
+      ++ eapply single_sub; auto.
+      ++ eapply v_single_xvx. auto. 
+    - exists (initial_finite_env ρ NE).
+      eexists; eauto. split. eauto.
+      rewrite denot_var.
+      rewrite access_fresh. simpl_env. auto.
+      rewrite access_fresh in vIn. auto. done.
+  + edestruct (APPLY_continuous NE vIn) as [ρ' [F SS]]; eauto.
+    eapply denot_monotone.
+    eapply denot_monotone.
+    exists ρ'. exists F.
+    rewrite denot_app. auto.
+  + pick fresh x.
+    rewrite (denot_abs x) in vIn. fsetdec.
+    move: (@Lambda_continuous _ _ NE v x vIn) => h.    
+    destruct h as [ρ' [Fρ' [S vvIn]]].
+    ++ intros V NEV NW.
+       move: (valid_nonempty_mem _ NEV) => [w h0]. 
+       eapply IH; eauto.
+    ++ eapply denot_monotone.
+    ++ exists ρ'. exists Fρ'. 
+       erewrite <- Forall2_dom in Fr. 2: eapply S.
+       rewrite (denot_abs x). fsetdec.
+       split; auto.
+  + edestruct (CONS_continuous vIn) as [ρ' [F SS]]; eauto.
+    eapply denot_monotone.
+    eapply denot_monotone.
+    exists ρ'. exists F.
+    rewrite denot_tcons. auto.
+Qed.
+
+
+(* ⟦⟧-continuous-⊆ *) 
+Lemma denot_continuous_sub {ρ t} : 
+  valid_env ρ
+  -> forall V, mem V ⊆ denot t ρ
+  -> exists ρ', exists (pf : finite_env ρ'),
+        ρ' ⊆e ρ  /\  (mem V ⊆ denot t ρ').
+Proof.
+  intros NE_ρ V VinEρ.
+  eapply continuous_In_sub; eauto.
+  eapply denot_monotone; eauto.
+  intros v InV.
+  eapply denot_continuous; auto.
+Qed.
+
+(* ⟦⟧-continuous-one *)
+Lemma denot_continuous_one { t ρ x } :
+  valid_env ρ 
+  -> x `notin` dom ρ 
+  -> continuous (fun D => denot (t ^ x) (x ~ D ++ ρ)).
+Proof.
+  intros NE_ρ Fr.
+  unfold continuous.
+  intros X E E_sub_denot NE_X.
+  edestruct (@denot_continuous_sub (x ~ X ++ ρ)) as 
+    [ρ' [pf [h1 h2]]]. 3: eauto.
+  + eapply extend_valid_env; eauto.
+  + eauto.
+  + inversion h1. subst. inversion pf. subst.
+    move: H6 => [D [S NN]].
+    exists D. split.
+    rewrite <- S. auto.
+    split. 
+    have SUB: Env.Forall2 Included (x ~ a1 ++ E1) (x ~ mem D ++ ρ).
+    econstructor; eauto. 
+    rewrite <- S. reflexivity.
+    rewrite <- SUB.
+    auto.
+    eapply valid_sub_valid_mem; eauto. rewrite <- S. auto.
+Qed.
+
+(*  Abstraction followed by Application is the identity ------------------- *)
+
+(* Λ-▪-id *)
+Lemma Λ_APPLY_id { F X } :
+  continuous F -> monotone F -> valid X
+  -> (Λ F) ▩ X ≃ F X.
+Proof. 
+  intros Fcont Fmono NEX.
+  split.
+  + intros w APP. inversion APP; subst. 
+    - inversion H.
+    - exfalso; eapply valid_not_wrong; eauto. 
+    - inversion H.
+      eapply (Fmono (mem V) X); eauto. 
+    - inversion H.
+    - destruct x; try done.
+    - destruct x; try done.
+  + intros w wInFX.
+    have M: mem (cons w nil) ⊆ F X. 
+    { intros d y. inversion y; subst. auto. done. }
+    move: (Fcont X (cons w nil) M NEX) => 
+    [ D [ DltX [ wInFD NED ]]].
+    move: NEX => [ [x h0] h1].
+    eapply BETA with (V:=D); eauto.
+    repeat split; eauto.
+    eapply Forall_sub_mem; eauto.
+Qed.
+
+
+(* Λ⟦⟧-▪-id *)
+Lemma Λ_denot_APPLY_id :
+  forall t ρ x X,
+    valid X
+    -> valid_env ρ
+    -> x `notin` dom ρ 
+    -> ((Λ (fun D => denot (t ^ x) (x ~ D ++ ρ))) ▩ X) ≃
+      denot (t ^ x) (x ~ X ++ ρ).
+Proof.
+  intros.
+  move: (@Λ_APPLY_id (fun D => denot (t ^ x) (x ~ D ++ ρ)) X) => h.
+  eapply h; auto.
+  +  (* continuity *)
+    eapply denot_continuous_one; auto.
+  + eapply denot_monotone_one; auto.
+    eapply ForallT_uniq; eauto.
+Qed.
