coq/denot/theory.v
@@ -1,0 +1,527 @@
+Require Import Coq.Logic.FunctionalExtensionality.
+Require Import Coq.Classes.RelationClasses.
+Require Coq.Relations.Relation_Definitions.
+Require Import Lia.
+
+Require Export lc.tactics.
+Require Import lc.scoped.
+
+Require Import structures.Structures.
+
+Import SetNotations.
+Local Open Scope set_scope.
+Import MonadNotation.
+Open Scope monad_scope.
+
+(* Definitions *)
+Require Import denot.definitions.
+
+(* Weakening & substitution for the definition of the denotation *)
+Require Import denot.denot.
+
+(* Operators preserve validity *)
+Require Import denot.valid_theory.
+
+(* Congruence: operators respect  *)
+Require Import denot.congruence_theory.
+
+(* Denotation function is continuous. *)
+Require Import denot.continuity.
+
+(* Denotation produces a consistent set *)
+Require Import denot.consistency.
+
+Import EnvNotations.
+Import LCNotations.
+Local Open Scope tm.
+
+(* ---- -------------------------------------- *)
+
+(* k∈℘k *)
+Lemma k_in_den_k : forall k, v_nat k ∈ NAT k.
+Proof. intros. reflexivity. Qed.
+
+Lemma k_in_den_k'_inv : forall k k', v_nat k ∈ NAT k' -> k = k'.
+Proof. intros. inversion H. done. Qed.
+
+Lemma v_in_den_k_inv :  forall v k, v ∈ NAT k -> v = v_nat k.
+Proof. intros. destruct v; inversion H. done. Qed.
+
+
+Lemma NAT_den {k} : NAT k ≃ ⌈ v_nat k ⌉.
+split. intros x In. destruct x; try done. inversion In. subst. constructor.
+intros x In. inversion In. cbn. auto. Qed.
+
+Lemma den_list : forall i j D, D ⊆ LIST (NAT i :: NAT j :: nil) ->
+                 forall x, x ∈ D -> x = v_list (v_nat i :: v_nat j :: nil).
+Proof.
+  intros.
+  specialize (H x H0).
+  destruct x; try done. 
+  destruct l; try done; inversion H; subst; clear H.
+  apply v_in_den_k_inv in H4. subst.
+  inversion H6. subst. clear H6.
+  apply v_in_den_k_inv in H2. subst.
+  inversion H4. subst.
+  reflexivity.
+Qed.
+
+Lemma CONS_LIST {k1 k2 } : CONS (NAT k1) (CONS (NAT k2) NIL) ≃ LIST (NAT k1 :: NAT k2 :: nil).
+Proof.
+  intros.
+  split.
+  + intros w In. destruct w; try done.
+    destruct l; try done.
+    destruct In as [x In]. apply v_in_den_k_inv in x.
+    destruct l; try done.
+    destruct In as [y In]. apply v_in_den_k_inv in y.
+    destruct l; try done. 
+    subst. cbn. 
+    econstructor; eauto. reflexivity. 
+    econstructor; eauto. reflexivity. 
+    cbv in In. inversion In.
+  + intros w In.
+    eapply den_list in In. 2: { reflexivity.  }
+    subst. 
+    econstructor; eauto using k_in_den_k.
+    econstructor; eauto using k_in_den_k.
+    econstructor.
+Qed.
+
+
+Lemma ADD_APPLY_LIST {i j} : 
+  ADD ▩ (LIST (NAT i :: NAT j :: nil)) ≃ NAT (i + j).
+Proof.
+  split.
+  + intros w APP. inversion APP; subst; clear APP.
+    all: cbn in H.
+    all: try done.
+    destruct w; try done.
+    - destruct H as [i0 [j0 [h0 h1]]]. subst.
+      move: (den_list _ _ _ H0 _ h0) => h1. inversion h1. subst. clear h1.
+      eapply k_in_den_k.
+    - destruct H as [H VV]. 
+      assert False. eapply H.
+      destruct V; try done. destruct H1. done.
+      move: (den_list _ _ _ H0 v ltac:(auto)) => h1. subst. 
+      eauto.
+      done.
+    - destruct x; try done.
+   + intros w wIn.
+     apply v_in_den_k_inv in wIn. subst.
+     eapply BETA with (V := v_list (v_nat i :: v_nat j :: nil) :: nil).
+     - cbn. eauto.
+     - intros x xIn. inversion xIn. subst.
+       cbn. eauto using k_in_den_k.
+       inversion H.
+     - cbn. split. eauto. unfold In, mem. intro h. inversion h. 
+       econstructor; eauto. done.
+Qed.
+
+Lemma ADD_APPLY_CONS {k1 k2} : 
+  (ADD ▩ CONS (NAT k1) (CONS (NAT k2) NIL)) ≃ NAT (k1 + k2).
+Proof.
+  rewrite CONS_LIST.
+  eapply ADD_APPLY_LIST.
+Qed. 
+
+Lemma CONS_APPLY_ZERO1 {D1 D2} : (CONS D1 D2 ▩ NAT 0) ⊆ D1.
+  intros w APP. inversion APP; try inversion H.
+  + subst.
+    apply v_in_den_k_inv in H0. inversion H0. subst.
+    destruct VS; simpl in H1. done. inversion H1. subst.
+    inversion H.
+    auto.
+  + destruct x; try done.
+  + destruct x; try done. 
+    apply v_in_den_k_inv in H0.  
+    exfalso; eapply H2; eauto.
+Qed.
+
+Lemma CONS_APPLY_ZERO2 {D1 D2 VS} : 
+  v_list VS ∈ D2 ->
+  D1 ⊆ (CONS D1 D2 ▩ NAT 0).
+Proof.
+  intros VV w In.
+  eapply PROJ with (k := 0)(VS := w :: VS); eauto using k_in_den_k.
+  econstructor; eauto.
+Qed. 
+
+Lemma CONS_APPLY_SUCC1 {D1 D2 k} : (CONS D1 D2 ▩ NAT (1 + k)) ⊆ (D2 ▩ NAT k).
+  intros w APP. inversion APP; try inversion H.
+  + subst.
+    apply v_in_den_k_inv in H0. inversion H0. subst.
+    destruct VS; simpl in H1. done. 
+    inversion H.
+    eapply PROJ; eauto using k_in_den_k.
+  + destruct x; try done.
+  + destruct x; try done.
+    exfalso; eapply H2; eauto.
+Qed.
+
+Lemma CONS_APPLY_SUCC2 {D1 D2 k w} : w ∈ D1 -> valid D2 -> (D2 ▩ NAT k) ⊆  (CONS D1 D2 ▩ NAT (1 + k)).
+Proof.
+  intros wIn [h1 h2]  v vIn.
+  inversion vIn; subst; try done.
+Abort.
+
+
+(* ---------------------------------------------------- *)
+
+(* Nonempty environments *)
+
+Lemma extend_nonempty_env {ρ x X} : 
+  x `notin` dom ρ ->
+  nonemptyT X -> 
+  nonempty_env ρ -> nonempty_env (x ~ X ++ ρ).
+Proof. intros Fr NEP NEX. eapply ForallT_cons; eauto. Qed.
+
+#[export] Hint Resolve extend_nonempty_env : core.
+
+(* ---------------------------------------------------------- *)
+
+(* https://github.com/jsiek/denotational_semantics/blob/master/agda/ISWIMPValue.agda *)
+
+Definition denot1 (t : tm) (ρ : Rho) : P Value.
+  remember (size_tm t) as n.
+  have GE: n >= size_tm t. subst. auto. clear Heqn.
+  move: t GE ρ.
+  induction (lt_wf n) as [n _ denot].
+  Print tm.
+  intros [ i | x | u | t | k | (* add *) | (* nil *) | t ] SZ; simpl in SZ.
+  all: intros ρ.
+  - exact ⌈ v_wrong ⌉.
+  - exact (ρ ⋅ x).
+  - move: (fresh_for (dom ρ \u fv_tm u)) => x.
+    have F : P Value -> P Value.
+    intro D.
+    have LT: size_tm (u ^ x) < n. {  autorewrite with lngen; lia. }
+    specialize (denot (size_tm (u ^ x)) LT (u ^ x) ltac:(auto) (x ~ D ++ ρ)).
+    exact denot.
+    exact (Λ F).
+  - move: (denot (size_tm t) ltac:(lia) t ltac:(lia) ρ) => t'.
+    move: (denot (size_tm u) ltac:(lia) u ltac:(lia) ρ) => u'.
+    exact (t' ▩ u').
+  - exact (NAT k). 
+  - exact ADD.
+  - exact NIL.    
+  - move: (denot (size_tm t) ltac:(lia) t ltac:(lia) ρ) => t'.
+    move: (denot (size_tm u) ltac:(lia) u ltac:(lia) ρ) => u'.
+    exact (CONS t' u').
+Defined. 
+
+(* ------------------------------------------------------- *)
+
+(* Soundness of reduction with respect to denotation *)
+(* ISWIMPValue.agda *)
+
+Ltac invert_value :=
+  repeat match goal with 
+    | [ H : value (_ _) |- _ ] => inversion H; clear H; subst
+    | [ H : listvalue (_ _) |- _ ] => inversion H; clear H; subst
+  end.
+
+
+(* The denotation of syntactic values is valid. *)
+Lemma denot_value_valid {t}{ρ} : 
+  fv_tm t [<=] dom ρ -> valid_env ρ 
+  -> (value t -> valid (denot t ρ)) * 
+      (listvalue t -> forall x, x ∈ (denot t ρ) -> { l & v_list l = x}).
+Proof. 
+  intros FV NEρ.
+  induction t.
+  all: split.
+  all: intros vv.
+  all: autorewrite with denot.
+  all: try solve [ assert False; invert_value; done].
+  + unfold nonempty_env in NEρ.
+    eapply (@ForallT_access _ ⌈ v_wrong ⌉ _ _) in NEρ.
+    2: instantiate (1:= x); auto.
+    destruct NEρ. split; auto.
+    simpl in FV. fsetdec.
+  + pick fresh x.
+    erewrite denot_abs with (x:=x); eauto.
+    eapply valid_Λ.
+  + eapply valid_NAT; eauto. 
+  + eapply valid_ADD; eauto.
+  + assert False. inversion vv. done.
+  + eapply valid_NIL; eauto.
+  + (* exists nil. cbv. econstructor. *)
+    intros x In. inversion In. exists nil. reflexivity.
+  + simpl in FV. 
+    move: (IHt1 ltac:(fsetdec)) => [ih11 _].
+    move: (IHt2 ltac:(fsetdec)) => [ih21 ih22].
+    have V2: value t2. invert_value. auto.
+    have LV: listvalue t2. invert_value. auto.
+    move: (ih21 V2) => [[v u] NW].
+    move: (ih22 LV v u) => [ll ii].
+    eapply valid_CONS; eauto. eapply ih11. invert_value. auto.
+    subst. eauto.
+  + simpl in FV. 
+    move: (IHt1 ltac:(fsetdec)) => [ih11 _].
+    move: (IHt2 ltac:(fsetdec)) => [ih21 ih22].
+    have V2: value t2. invert_value. auto.
+    have LV: listvalue t2. invert_value. auto.
+    move: (ih21 V2) => [[v u] NW].
+    move: (ih22 LV v u) => [ll ii].
+    subst.
+    intros x CC. 
+    destruct x; try done.
+    exists l. reflexivity.
+Qed.     
+
+Lemma value_nonempty {t}{ρ} : 
+  fv_tm t [<=] dom ρ -> valid_env ρ -> value t -> valid (denot t ρ).
+Proof. 
+  intros.
+  eapply denot_value_valid; eauto.
+Qed. 
+
+Lemma soundness: 
+  forall t u, 
+    full_reduction t u ->
+    forall ρ,
+    scoped t ρ ->
+    scoped u ρ ->
+    valid_env ρ ->
+    denot t ρ ≃ denot u ρ.
+Proof.
+  intros t u RED. 
+  induction RED; intros ρ SCt SCu NE.
+  - (* beta *)
+    destruct SCt as [FV U lc]. inversion lc. subst.
+    simpl in FV.
+    rewrite denot_app.
+    pick fresh x.
+    erewrite denot_abs with (x:=x).
+    rewrite Λ_denot_APPLY_id.
+    eapply value_nonempty; auto.
+    fsetdec.
+    auto.
+    fsetdec.
+    rewrite (subst_tm_intro x t v); auto.
+    replace ρ with (nil ++ ρ) at 3.
+    rewrite <- subst_denot with (ρ1 := nil). reflexivity.
+    simpl_env.
+    econstructor; eauto. 
+    rewrite fv_tm_open_tm_wrt_tm_upper. simpl. fsetdec.
+    inversion H; eauto.
+    econstructor; eauto. 
+    fsetdec.
+    reflexivity.
+    fsetdec.
+  - (* abs-cong *)
+    pick fresh x.
+    repeat erewrite denot_abs with (x:=x); try fsetdec.
+    specialize (H0 x ltac:(auto)).
+    eapply Λ_ext.
+    intros X NEX.
+    eapply H0.
+    have F1 : x `notin` dom ρ \u fv_tm t. fsetdec.
+    eapply (scoped_abs_inv _ x _ X _ F1 SCt).
+    have F2 : x `notin` dom ρ \u fv_tm t'. fsetdec.
+    eapply (scoped_abs_inv _ x _ X _ F2 SCu).
+    eapply extend_valid_env.
+    fsetdec.
+    eauto.
+    eauto.
+  - have SC1: scoped t ρ. eapply scoped_app_inv1; eauto.
+    have SC2: scoped t' ρ. eapply scoped_app_inv1; eauto.
+    have SC3: scoped u ρ. eapply scoped_app_inv2; eauto.
+    repeat rewrite denot_app.
+    eapply APPLY_cong; eauto.
+    reflexivity.
+  - have SC1: scoped t ρ.  eapply scoped_app_inv1; eauto.
+    have SC2: scoped u ρ.  eapply scoped_app_inv2; eauto.
+    have SC3: scoped u' ρ.  eapply scoped_app_inv2; eauto.
+    repeat rewrite denot_app.
+    eapply APPLY_cong; eauto.
+    reflexivity.
+  - repeat rewrite denot_tcons; eauto.
+    eapply CONS_cong; eauto.
+    have SC1: scoped t ρ.  eapply scoped_tcons_inv1; eauto.
+    have SC2: scoped u ρ.  eapply scoped_tcons_inv2; eauto.
+    have SC3: scoped t' ρ.  eapply scoped_tcons_inv1; eauto.
+    eapply IHRED; eauto.
+    reflexivity.
+  - repeat rewrite denot_tcons.
+    have SC1: scoped t ρ.  eapply scoped_tcons_inv1; eauto.
+    have SC2: scoped u ρ.  eapply scoped_tcons_inv2; eauto.
+    have SC3: scoped u' ρ.  eapply scoped_tcons_inv2; eauto.
+    rewrite IHRED; eauto.
+    reflexivity.
+  - autorewrite with denot.
+    destruct SCt. simpl in s.
+    move: (@denot_value_valid w ρ ltac:(fsetdec) NE) => [w1 w2].
+    move: (w1 (sv_list _ H0)) => [[uu ss] NW].
+    move: (w2 H0 uu ss) => [ll tt]. subst.
+    
+    split. eapply CONS_APPLY_ZERO1.
+    eapply CONS_APPLY_ZERO2; eauto.
+
+  - (* prj_suc *)
+    autorewrite with denot.
+    split.
+    + eapply CONS_APPLY_SUCC1.
+    + intros x In.
+      destruct SCt. simpl in s.
+      move: (@denot_value_valid v ρ ltac:(fsetdec) NE) => [h1 h2].
+      move: (@denot_value_valid w ρ ltac:(fsetdec) NE) => [w1 w2].
+      move: (h1 H) => [[vv rr] NW]. clear h1 h2.
+      move: (w1 (sv_list _ H0)) => [[uu ss] NW2].
+      move: (w2 H0) => mm.  
+      inversion In; try done; subst.
+      ++ move: (mm _ H1) => [o OO]. done.
+      ++ move: (mm _ H1) => [o OO]. done.
+      ++ move: (mm _ H1) => [o OO]. 
+      inversion H2. subst.
+      eapply PROJ. instantiate (1 := (vv :: VS)).
+      econstructor; eauto.
+      instantiate (1:= (1 + k0)). econstructor.
+      simpl.
+      auto.
+      ++ move: (mm _ H1) => [o OO].  subst. simpl in H3; done.
+      ++ destruct x0; try done. exfalso.  eapply H4; eauto. 
+  - (* add *) 
+    autorewrite with denot.
+    eapply ADD_APPLY_CONS; eauto.
+Qed.
+
+
+(* --------------------------------------------------------------- *)
+
+(* Example semantics *)
+
+
+Definition tm_Id : tm := abs (var_b 0).
+
+Lemma denot_Id {v} : success v  -> (v :: nil ↦ v) ∈ denot tm_Id nil.
+Proof.
+  intro NE.
+  pick fresh x.
+  rewrite (denot_abs x); simpl; auto.
+  cbn.
+  destruct (x == x); try done.
+  cbn. split. left. auto. 
+  econstructor; eauto. done.
+Qed. 
+
+
+Lemma denot_Id_inv : forall x ρ, x ∈ denot tm_Id ρ ->
+                          forall w,  Consistent x (w :: nil ↦ w).
+Proof.
+  intros x ρ.
+  unfold tm_Id. 
+  pick fresh y.
+  rewrite (denot_abs y); auto.
+  intro h. 
+  destruct x; try done.
+  move: h => [h0 [h1 h2]].
+  cbn in h0. rewrite eq_dec_refl in h0.
+  intros w.
+  destruct (dec_con x w). eauto.
+  eapply c_map1.
+  exists x. exists w.
+  
+  repeat split; eauto. 
+  unfold In. eauto.
+Qed.
+
+Definition tm_Delta : tm := abs (app (var_b 0) (var_b 0)).
+
+
+#[global] Hint Rewrite access_eq_var : lngen.
+
+Lemma wrong_not_successful {l}: 
+  Forall success l -> v_wrong ∈ mem l -> False.
+Proof. 
+  induction l; intros h1 h2. done.
+  inversion h1. subst. 
+  inversion h2. subst. done.
+  eauto.
+Qed.
+
+Lemma denot_Delta_inv :
+  forall x, x ∈ denot tm_Delta nil -> 
+       exists v w, Consistent x (((v :: nil ↦ w) :: v :: nil) ↦ w).
+Proof.
+  intro x. unfold tm_Delta.
+  pick fresh y.
+  rewrite (denot_abs y); auto.
+  cbn. rewrite eq_dec_refl.
+  destruct x; try done.
+  move=> [h0 [h1 h2]].
+  - inversion h0; subst; try done.
+    + exfalso. eapply wrong_not_successful; eauto.
+    + exfalso. eapply wrong_not_successful; eauto.
+    + exists (l ↦ x). exists x.
+      eapply c_map2. reflexivity.
+    + exists (l ↦ x). exists x.
+      eapply c_map2. reflexivity.
+    + exists (v_nat 0). exists v_wrong. eauto.
+    + exists (v_nat 0). exists v_wrong. eauto.
+  - cbn. intros.
+      exists v_fun. exists v_fun. eauto.
+Qed.
+
+Lemma denot_Delta : forall (v w : Value), success v ->
+    (((v :: nil ↦ w) :: v :: nil) ↦ w) ∈ denot tm_Delta nil.
+Proof.
+  intros v w NW.
+  pick fresh x.
+  unfold tm_Delta.
+  rewrite (denot_abs x); auto.
+  cbn. rewrite eq_dec_refl.
+  split. 2: { unfold valid_mem. split. intro h. done. 
+              econstructor; eauto. done. }
+  cbv.
+  eapply BETA with (V := v :: nil).
+  unfold In. left. auto.
+  rewrite -> mem_singleton. 
+  intros x0 II. inversion II. subst. cbv. right. left. auto.
+  unfold valid_mem.
+  split; eauto.
+  intro h. done. 
+Qed.
+  
+
+Definition tm_Omega : tm := app tm_Delta tm_Delta.
+
+Lemma denot_Omega : forall v, not (v ∈ denot tm_Omega nil).
+Proof.
+unfold tm_Omega.
+rewrite denot_app.
+intro v.
+intro h.
+inversion h; subst; clear h.
++ apply denot_Delta_inv in H.
+  move: H => [v [w C]]. inversion C.
++ apply denot_Delta_inv in H.
+  move: H => [v [w C]]. inversion C.
++ apply denot_Delta_inv in H.
+  move: H => [v1 [w2 C]]. 
+  inversion C; subst.
+Admitted.
+
+(* A term with an unbound variable has no value. *)
+Definition tm_Wrong : tm := app (var_b 1) (var_b 0).
+
+Lemma denot_Wrong : v_wrong ∈ denot tm_Wrong nil.
+Proof.
+  unfold tm_Wrong.
+  rewrite denot_app.
+  repeat rewrite denot_var_b.
+  eapply FUNWRONG.
+  auto.
+Qed.  
+
+
+
+
+(* Λ  \Lambda
+   ▩  \squarecrossfill 
+   ↦  \mapsto  
+   ⤇ \Mapsto  
+   ●  \CIRCLE 
+   ⊆  \subseteq   (Included)
+*)
