coq/lc/scoped.v
@@ -7,8 +7,8 @@ Require Import Coq.Classes.RelationClasses.
 Require Coq.Relations.Relation_Definitions.
 Require Import Lia.
 
-Require Export lc.tactics.
-Require Import lc.Env.
+Require Export tactics.
+Require Import structures.Env.
 
 Import LCNotations.
 Open Scope tm.
