coq/structures/Structures.v
@@ -1,0 +1,5 @@
+Require Export structures.Container.
+Require Export structures.Sets.
+Require Export structures.List.
+Require Export structures.Env.
+Require Export structures.Monad.
